- completed more of the proof for conditional assignment. - started writing loop invariant

specs/verif_hmac_drbg_update.v
@@ -5,6 +5,45 @@ Require Import floyd.sublist.
 
 Require Import hmac_drbg.
 Require Import spec_hmac_drbg.
+Require Import HMAC_DRBG_update.
+Require Import sha.HMAC256_functional_prog.
+
+Fixpoint HMAC_DRBG_update_round (HMAC: list Z -> list Z -> list Z) (provided_data K V: list Z) (sep: Z) (round: nat): (list Z * list Z) :=
+  match round with
+    | O => (K, V)
+    | S round' =>
+      let K := HMAC (V ++ [sep] ++ provided_data) K in
+      let V := HMAC V K in
+      HMAC_DRBG_update_round HMAC provided_data K V (sep + 1) round'
+  end.
+
+Definition HMAC_DRBG_update_concrete (HMAC: list Z -> list Z -> list Z) (provided_data K V: list Z): (list Z * list Z) :=
+  let rounds := match provided_data with
+                  | [] => 1%nat
+                  | _ => 2%nat
+                end in
+  HMAC_DRBG_update_round HMAC provided_data K V 0 rounds.
+
+Theorem HMAC_DRBG_update_concrete_correct:
+  forall HMAC provided_data K V, HMAC_DRBG_update HMAC provided_data K V = HMAC_DRBG_update_concrete HMAC provided_data K V.
+Proof.
+  intros.
+  destruct provided_data; reflexivity.
+Qed.
+
+Definition update_loop_invariant ctx sep provided_data old_key old_value state_abs state i key value :=
+  (*
+  EX i: _, EX key: _, EX value: _,
+   *)
+  PROP  ((key, value) = HMAC_DRBG_update_round HMAC256 provided_data old_key old_value 0 i)
+  LOCAL  (
+    lvar _sep (tarray tuchar 1) sep
+         )
+  SEP  (
+  `(data_at Tsh (tarray tuchar 1) [Vint (Int.repr (Z.of_nat i))] sep);
+  `(data_at Tsh t_struct_hmac256drbg_context_st state ctx);
+  `(hmac256drbg_relate (hmac256drbgabs_update_key (hmac256drbgabs_update_value state_abs value) key) state)
+  ).
 
 Lemma body_hmac_drbg_update: semax_body HmacDrbgVarSpecs HmacDrbgFunSpecs 
        f_mbedtls_hmac_drbg_update hmac_drbg_update_spec.
@@ -20,7 +59,7 @@ Proof.
   forward_call tt md_len.
 
   (* rounds = ( additional != NULL && add_len != 0 ) ? 2 : 1; *)
-  remember (if eq_dec add_len 0 then false else if eq_dec additional nullval then true else false) as non_empty_additional.
+  remember (if eq_dec add_len 0 then false else if eq_dec additional nullval then false else true) as non_empty_additional.
   forward_if (
       PROP  ()
       LOCAL  (temp _md_len md_len; lvar _K (tarray tuchar 32) K;
@@ -50,8 +89,22 @@ Proof.
       solve_valid_pointer.
     }
     entailer!.
-    rewrite <- H3.
-    admit (* TODO *).
+    clear - H3 H1 TC.
+    rewrite Zlength_map in *.
+    destruct (eq_dec (Zlength contents) 0) as [zlength_eq | zlength_neq].
+    assert (contra: False) by (apply H1; apply zlength_eq); inversion contra.
+    destruct additional'; try solve [inversion TC]. 
+    {
+      inv TC.
+      destruct (eq_dec (Vint Int.zero) nullval) as [additional_eq | additional_neq].
+      auto.
+      assert (contra: False) by (apply additional_neq; reflexivity); inversion contra.
+    }
+    {
+      destruct (eq_dec (Vptr b i) nullval) as [additional_eq | additional_neq].
+      inversion additional_eq.
+      auto.
+    }
   }
 
   {
@@ -66,7 +119,6 @@ Proof.
       lvar _sep (tarray tuchar 1) sep;
       lvar _info (Tstruct _mbedtls_md_info_t noattr) info;
       temp _additional additional; temp _add_len (Vint (Int.repr add_len));
-      temp 126%positive (Val.of_bool non_empty_additional);
       temp 127%positive (if non_empty_additional then (Vint (Int.repr 2)) else (Vint (Int.repr 1)))
              )
       SEP  (`(data_at_ Tsh (tarray tuchar 32) K);
@@ -86,5 +138,10 @@ Proof.
     forward.
     entailer!.
   }
+  forward.
+
+  (* sep[0] = 0 *)
+  forward.
+
   forward.
 Admitted.
